<section xml:id="sec-logical-equivalence">
    <title>Logical Equivalences</title>
    <objectives xml:id="obj-logical-equivalences">
  <title>Goals for This Section</title>
  <ol>
    <li>
      Define <term>logical equivalence</term> and use truth tables to determine whether
      two statements are logically equivalent.
    </li>
    <li>
      Apply common equivalence laws, including <term>De Morgan’s Laws </term> and the
      double-negation law, to rewrite statements more simply.
    </li>
    <li>
      Learn how to negate statements involving conjunctions, disjunctions, and conditionals.
    </li>
  </ol>
</objectives>

<definition xml:id="def-lequivalence">
    <statement>
<p>
  Two statements are <term>logically equivalent</term> if they have the same truth value
  for every possible assignment of truth values to their variables. Equivalently, their truth tables have
  identical final columns. We use <m>\equiv</m> to denote logical equivalence between statements.
</p>

    </statement>
</definition>  
<example xml:id="example-double-negation-equivalence">
  <title><m> p \equiv \lnot(\lnot p)</m></title>

  <p>
    The following truth table shows that the statements
    <m>p</m> and <m>\lnot(\lnot p)</m> always have the same truth value.
    Therefore, they are logically equivalent,  thus 
    <me>
    p \equiv \lnot(\lnot p)
  </me>
  </p>

  <table>
    <title>Truth Table for <m>p</m> and <m>\lnot(\lnot p)</m></title>
    <tabular halign="center">
      <row header="yes" bottom="minor">
        <cell><m>p</m></cell>
        <cell><m>\lnot p</m></cell>
        <cell><m>\lnot(\lnot p)</m></cell>
      </row>
      <row>
        <cell>T</cell>
        <cell>F</cell>
        <cell>T</cell>
      </row>
      <row>
        <cell>F</cell>
        <cell>T</cell>
        <cell>F</cell>
      </row>
    </tabular>
  </table>

  <p>
    Since the columns for <m>p</m> and <m>\lnot(\lnot p)</m> are identical,
    we conclude that <m>p \equiv \lnot(\lnot p)</m>.
  </p>
</example>
<example xml:id="example-disjunction-commutative">
  <title><m>p \lor q \equiv q \lor p</m></title>

  <p>
    The following truth table shows that the statements
    <m>p \lor q</m> and <m>q \lor p</m> always have the same truth value.
    Therefore, they are logically equivalent.
  </p>

  <table>
    <title>Truth Table for <m>p \lor q</m> and <m>q \lor p</m></title>
    <tabular halign="center">
      <row header="yes" bottom="minor">
        <cell><m>p</m></cell>
        <cell><m>q</m></cell>
        <cell><m>p \lor q</m></cell>
        <cell><m>q \lor p</m></cell>
      </row>
      <row>
        <cell>T</cell>
        <cell>T</cell>
        <cell>T</cell>
        <cell>T</cell>
      </row>
      <row>
        <cell>T</cell>
        <cell>F</cell>
        <cell>T</cell>
        <cell>T</cell>
      </row>
      <row>
        <cell>F</cell>
        <cell>T</cell>
        <cell>T</cell>
        <cell>T</cell>
      </row>
      <row>
        <cell>F</cell>
        <cell>F</cell>
        <cell>F</cell>
        <cell>F</cell>
      </row>
    </tabular>
  </table>

  <p>
    Since the columns for <m>p \lor q</m> and <m>q \lor p</m> are identical,
    we conclude that <m>p \lor q \equiv q \lor p</m>.
  </p>
</example>
<exercise xml:id="ex-equivalence-implication-disjunction">
  <title><me>p \to q \equiv (\lnot p)\lor q</me></title>

  <statement>
    <p>
      Show that <m>p \to q</m> and <m>(\lnot p)\lor q</m> are logically equivalent.
    </p>
  </statement>

  <solution>
    <p>
      We compare the truth values of <m>p \to q</m> and <m>(\lnot p)\lor q</m>
      for all possible truth values of <m>p</m> and <m>q</m>.
    </p>

    <table>
      <title>Truth Table Comparison</title>
      <tabular halign="center">
        <row header="yes" bottom="minor">
          <cell><m>p</m></cell>
          <cell><m>q</m></cell>
          <cell><m>\lnot p</m></cell>
          <cell><m>(\lnot p)\lor q</m></cell>
          <cell><m>p \to q</m></cell>
        </row>

        <row>
          <cell>T</cell><cell>T</cell><cell>F</cell><cell>T</cell><cell>T</cell>
        </row>
        <row>
          <cell>T</cell><cell>F</cell><cell>F</cell><cell>F</cell><cell>F</cell>
        </row>
        <row>
          <cell>F</cell><cell>T</cell><cell>T</cell><cell>T</cell><cell>T</cell>
        </row>
        <row>
          <cell>F</cell><cell>F</cell><cell>T</cell><cell>T</cell><cell>T</cell>
        </row>
      </tabular>
    </table>

    <p>
      The columns for <m>p \to q</m> and <m>(\lnot p)\lor q</m> are identical,
      so the two statements are logically equivalent.
      Thus, <m>p \to q \equiv (\lnot p)\lor q</m>.
    </p>
  </solution>
</exercise>
<exercise xml:id="ex-equivalence-conditional-reversal">
  <title>Logical Equivalence of Conditionals</title>

  <statement>
    <p>
      Determine whether the statements <m>p \to q</m> and <m>q \to p</m>
      are logically equivalent. Justify your answer by constructing a truth table.
    </p>
  </statement>

  <solution>
    <p>
      We compare the truth values of <m>p \to q</m> and <m>q \to p</m>
      for all possible truth values of <m>p</m> and <m>q</m>.
    </p>

    <table>
      <title>Truth Table Comparison</title>
      <tabular halign="center">
        <row header="yes" bottom="minor">
          <cell><m>p</m></cell>
          <cell><m>q</m></cell>
          <cell><m>p \to q</m></cell>
          <cell><m>q \to p</m></cell>
        </row>

        <row>
          <cell>T</cell>
          <cell>T</cell>
          <cell>T</cell>
          <cell>T</cell>
        </row>
        <row>
          <cell>T</cell>
          <cell>F</cell>
          <cell>F</cell>
          <cell>T</cell>
        </row>
        <row>
          <cell>F</cell>
          <cell>T</cell>
          <cell>T</cell>
          <cell>F</cell>
        </row>
        <row>
          <cell>F</cell>
          <cell>F</cell>
          <cell>T</cell>
          <cell>T</cell>
        </row>
      </tabular>
    </table>

    <p>
      Since the columns for <m>p \to q</m> and <m>q \to p</m> differ,
      the two statements are <term>not</term> logically equivalent.
    </p>
  </solution>
</exercise>
<remark xml:id="remark-demorgan-laws">
  <title>De Morgan’s Laws</title>

  <p>
    De Morgan’s Laws describe how negation interacts with conjunction
    and disjunction. They state that negating a compound statement changes
    <term>and</term> to <term>or</term>, and <term>or</term> to <term>and</term>,
    while negating each individual statement.
  </p>

  <example xml:id="example-demorgan-and">
    <title>Negation of a Conjunction</title>
    <p>
      The statement <m>\lnot(p \land q)</m> is logically equivalent to
      <m>(\lnot p)\lor(\lnot q)</m>.
    </p>
    <md>
      \lnot(p \land q) \equiv (\lnot p)\lor(\lnot q)
    </md>
      <p>
    We use truth tables to verify this De Morgan’s Law by comparing the truth values
    of each pair of statements.
  </p>


  <table>
    <title>Truth Table for <m>\lnot(p \land q)</m> and <m>(\lnot p)\lor(\lnot q)</m></title>
    <tabular halign="center">
      <row header="yes" bottom="minor">
        <cell><m>p</m></cell>
        <cell><m>q</m></cell>
        <cell><m>p \land q</m></cell>
        <cell><m>\lnot(p \land q)</m></cell>
        <cell><m>\lnot p</m></cell>
        <cell><m>\lnot q</m></cell>
        <cell><m>(\lnot p)\lor(\lnot q)</m></cell>
      </row>

      <row><cell>T</cell><cell>T</cell><cell>T</cell><cell>F</cell><cell>F</cell><cell>F</cell><cell>F</cell></row>
      <row><cell>T</cell><cell>F</cell><cell>F</cell><cell>T</cell><cell>F</cell><cell>T</cell><cell>T</cell></row>
      <row><cell>F</cell><cell>T</cell><cell>F</cell><cell>T</cell><cell>T</cell><cell>F</cell><cell>T</cell></row>
      <row><cell>F</cell><cell>F</cell><cell>F</cell><cell>T</cell><cell>T</cell><cell>T</cell><cell>T</cell></row>
    </tabular>
  </table>

  <p>
    The columns for <m>\lnot(p \land q)</m> and <m>(\lnot p)\lor(\lnot q)</m>
    are identical, so
    <m>\lnot(p \land q)\equiv(\lnot p)\lor(\lnot q)</m>.
  </p>
  </example>

  <example xml:id="example-demorgan-or">
    <title>Negation of a Disjunction</title>
    <p>
      The statement <m>\lnot(p \lor q)</m> is logically equivalent to
      <m>(\lnot p)\land(\lnot q)</m>.
    </p>
    <md>
      \lnot(p \lor q) \equiv (\lnot p)\land(\lnot q)
    </md>
     <table>
    <title>Truth Table for <m>\lnot(p \lor q)</m> and <m>(\lnot p)\land(\lnot q)</m></title>
    <tabular halign="center">
      <row header="yes" bottom="minor">
        <cell><m>p</m></cell>
        <cell><m>q</m></cell>
        <cell><m>p \lor q</m></cell>
        <cell><m>\lnot(p \lor q)</m></cell>
        <cell><m>\lnot p</m></cell>
        <cell><m>\lnot q</m></cell>
        <cell><m>(\lnot p)\land(\lnot q)</m></cell>
      </row>

      <row><cell>T</cell><cell>T</cell><cell>T</cell><cell>F</cell><cell>F</cell><cell>F</cell><cell>F</cell></row>
      <row><cell>T</cell><cell>F</cell><cell>T</cell><cell>F</cell><cell>F</cell><cell>T</cell><cell>F</cell></row>
      <row><cell>F</cell><cell>T</cell><cell>T</cell><cell>F</cell><cell>T</cell><cell>F</cell><cell>F</cell></row>
      <row><cell>F</cell><cell>F</cell><cell>F</cell><cell>T</cell><cell>T</cell><cell>T</cell><cell>T</cell></row>
    </tabular>
  </table>

  <p>
    Since the final columns match, we conclude that
    <m>\lnot(p \lor q)\equiv(\lnot p)\land(\lnot q)</m>.
  </p>
  </example>

</remark>

<subsection xml:id="subsec-exercises-logical-equivalence">
  <title>Exercises</title>

  <p>
    Determine whether each pair of statements is logically equivalent.  Justify your
    answer by using truth tables.
  </p>

  <question xml:id="q-equiv-a">
    <statement>
      <p>
        Determine whether <m>p\lor(p\land q)</m> and <m>p</m> are logically equivalent.
      </p>
    </statement>
    <solution>
      <table>
        <title>Truth Table for <m>p\lor(p\land q)</m> and <m>p</m></title>
        <tabular halign="center">
          <row header="yes" bottom="minor">
            <cell><m>p</m></cell>
            <cell><m>q</m></cell>
            <cell><m>p\land q</m></cell>
            <cell><m>p\lor(p\land q)</m></cell>
            <cell><m>p</m></cell>
          </row>
          <row><cell>T</cell><cell>T</cell><cell>T</cell><cell>T</cell><cell>T</cell></row>
          <row><cell>T</cell><cell>F</cell><cell>F</cell><cell>T</cell><cell>T</cell></row>
          <row><cell>F</cell><cell>T</cell><cell>F</cell><cell>F</cell><cell>F</cell></row>
          <row><cell>F</cell><cell>F</cell><cell>F</cell><cell>F</cell><cell>F</cell></row>
        </tabular>
      </table>
      <p>
        The final two columns are identical, so <m>p\lor(p\land q)\equiv p</m>.
      </p>
    </solution>
  </question>

  <question xml:id="q-equiv-b">
    <statement>
      <p>
        Determine whether <m>\lnot(p\lor q)</m> and <m>(\lnot p)\lor(\lnot q)</m>
        are logically equivalent.
      </p>
    </statement>
    <solution>
      <table>
        <title>Truth Table for <m>\lnot(p\lor q)</m> and <m>(\lnot p)\lor(\lnot q)</m></title>
        <tabular halign="center">
          <row header="yes" bottom="minor">
            <cell><m>p</m></cell>
            <cell><m>q</m></cell>
            <cell><m>p\lor q</m></cell>
            <cell><m>\lnot(p\lor q)</m></cell>
            <cell><m>\lnot p</m></cell>
            <cell><m>\lnot q</m></cell>
            <cell><m>(\lnot p)\lor(\lnot q)</m></cell>
          </row>
          <row><cell>T</cell><cell>T</cell><cell>T</cell><cell>F</cell><cell>F</cell><cell>F</cell><cell>F</cell></row>
          <row><cell>T</cell><cell>F</cell><cell>T</cell><cell>F</cell><cell>F</cell><cell>T</cell><cell>T</cell></row>
          <row><cell>F</cell><cell>T</cell><cell>T</cell><cell>F</cell><cell>T</cell><cell>F</cell><cell>T</cell></row>
          <row><cell>F</cell><cell>F</cell><cell>F</cell><cell>T</cell><cell>T</cell><cell>T</cell><cell>T</cell></row>
        </tabular>
      </table>
      <p>
        The columns for <m>\lnot(p\lor q)</m> and <m>(\lnot p)\lor(\lnot q)</m>
        are <term>not</term>identical, so they are logically equivalent.
      </p>
    </solution>
  </question>

  <question xml:id="q-equiv-c">
    <statement>
      <p>
        Determine whether <m>\lnot(p\to q)</m> and <m>(\lnot p)\to(\lnot q)</m>
        are logically equivalent.
      </p>
    </statement>
    <solution>
      <table>
        <title>Truth Table for <m>\lnot(p\to q)</m> and <m>(\lnot p)\to(\lnot q)</m></title>
        <tabular halign="center">
          <row header="yes" bottom="minor">
            <cell><m>p</m></cell>
            <cell><m>q</m></cell>
            <cell><m>p\to q</m></cell>
            <cell><m>\lnot(p\to q)</m></cell>
            <cell><m>\lnot p</m></cell>
            <cell><m>\lnot q</m></cell>
            <cell><m>(\lnot p)\to(\lnot q)</m></cell>
          </row>
          <row><cell>T</cell><cell>T</cell><cell>T</cell><cell>F</cell><cell>F</cell><cell>F</cell><cell>T</cell></row>
          <row><cell>T</cell><cell>F</cell><cell>F</cell><cell>T</cell><cell>F</cell><cell>T</cell><cell>T</cell></row>
          <row><cell>F</cell><cell>T</cell><cell>T</cell><cell>F</cell><cell>T</cell><cell>F</cell><cell>F</cell></row>
          <row><cell>F</cell><cell>F</cell><cell>T</cell><cell>F</cell><cell>T</cell><cell>T</cell><cell>T</cell></row>
        </tabular>
      </table>
      <p>
        The columns for <m>\lnot(p\to q)</m> and <m>(\lnot p)\to(\lnot q)</m> are not identical
        (for example, when <m>p=F</m> and <m>q=T</m>), so the statements are not logically equivalent.
      </p>
    </solution>
  </question>

</subsection>

<subsection xml:id="subsec-negating-statements">
  <title>Negating Statements</title>

  <p>
    Negating a statement means forming a new statement that is true exactly when
    the original statement is false. For compound statements, negation must be
    handled carefully.
  </p>

  <p>
    In particular, negating conjunctions and disjunctions follows
    <term>De Morgan’s Laws</term>, which were justified earlier using truth tables.
    See <xref ref="remark-demorgan-laws"/> for the formal statements.
  </p>

  <p>
    Negating conditional statements behaves differently and is a common source of
    confusion. The difference between a conditional and its reversal was explored
    in <xref ref="ex-equivalence-conditional-reversal"/>.
  </p>

  <exercise xml:id="ex-negating-english">
    <title>Negate the following Statements in English</title>

   

    <task xml:id="task-negate-simple">
      <statement>
        <p>We enjoy MATH.</p>
      </statement>
      <solution>
        <p>
          We do not enjoy MATH.
        </p>
      </solution>
    </task>

    <task xml:id="task-negate-conjunction">
      <statement>
        <p>We enjoy MATH and pizza.</p>
      </statement>
      <solution>
        <p>
          We do not enjoy MATH or we do not enjoy pizza.
        </p>
      </solution>
    </task>

    <task xml:id="task-negate-disjunction">
      <statement>
        <p>We enjoy MATH or pizza.</p>
      </statement>
      <solution>
        <p>
          We do not enjoy MATH and we do not enjoy pizza.
        </p>
      </solution>
    </task>
    <task xml:id="task-negate-conditional">
      <statement>
        <p>If we enjoy MATH, then we enjoy pizza.</p>
      </statement>
      <solution>
        <p>
          We enjoy MATH and we don't enjoy pizza.
        </p>
      </solution>
    </task>
  </exercise>

  <p>
    These examples illustrate how negation interacts with <term>and</term>,
    <term>or</term>, and <term>if, then </term>. This behavior is precisely described by De Morgan’s Laws.
  </p>

</subsection>

<subsection xml:id="subsec-exercise">
  <title>Exercise</title>


  <question xml:id="q-negate-conditional-a">
    <statement>
      <p>
        Find the negation of: "If you say “I do”, then you will be happy for the rest of your life."
      </p>
    </statement>
    <solution>
      <p>
        You say “I do” and you will not be happy for the rest of your life.
      </p>
    </solution>
  </question>

  <question xml:id="q-negate-conditional-b">
    <statement>
      <p>
      Find the negation of:  "I’ll be surprised if that is an authentic Persian rug."
      </p>
    </statement>
    <solution>
      <p>
        I am not surprised and that is an authentic Persian rug.
      </p>
    </solution>
  </question>

<!-- Question 1 -->
  <question xml:id="q-negation-joe">
    <statement>
      <p>
     "Joe tells you that he is an actor and went to India last summer.
        You know that he is lying. What compound statement about Joe is true?
      </p>
    </statement>
    <solution>
      <p>
        Joe is not an actor or he did not go to India last summer.
      </p>
    </solution>
  </question>

  <!-- Question 2 -->
  <question xml:id="q-simplify-demorgan">
    <statement>
      <p>
        Simplify the expression <m>\lnot[(\lnot p)\land q]</m> using De Morgan’s Laws
        and the double negation.
      </p>
    </statement>
    <solution>
      <p>
        By De Morgan’s Law,
        <m>\lnot[(\lnot p)\land q]\equiv \lnot(\lnot p)\lor \lnot q</m>.
        Using double negation, this simplifies to
        <m>p\lor \lnot q</m>.
      </p>
    </solution>
  </question>
<question xml:id="q-simplify-demorgan-2">
  <statement>
    <p>
      Simplify the expression <m>\lnot(p\lor \lnot q)</m> using De Morgan’s Laws
      and the double negation.
    </p>
  </statement>
  <solution>
    <p>
      By De Morgan’s Law,
      <m>\lnot(p\lor \lnot q)\equiv \lnot p \land \lnot(\lnot q)</m>.
      Using double negation, this simplifies to
      <m>\lnot p \land q</m>.
    </p>
  </solution>
</question>

<question xml:id="q-simplify-demorgan-3">
  <statement>
    <p>
      Simplify the expression <m>\lnot[(p\land q)\lor r]</m> using De Morgan’s Laws.
    </p>
  </statement>
  <solution>
    <p>
      By De Morgan’s Law,
      <m>\lnot[(p\land q)\lor r]\equiv \lnot(p\land q)\land \lnot r</m>.
      Applying De Morgan’s Law again,
      <m>\lnot(p\land q)\equiv \lnot p \lor \lnot q</m>.
      Thus, the expression simplifies to
      <m>(\lnot p \lor \lnot q)\land \lnot r</m>.
    </p>
  </solution>
</question>
<question xml:id="q-simplify-conditional-demorgan">
  <statement>
    <p>
      Simplify the expression <m>\lnot(p \to q)</m> using logical equivalence.
    </p>
  </statement>
  <solution>
    <p>
      First rewrite the conditional using logical equivalence:
      <m>p \to q \equiv \lnot p \lor q</m>.
    </p>

    <p>
      Substituting, we obtain
      <m>\lnot(\lnot p \lor q)</m>.
      By De Morgan’s Law, this is equivalent to
      <m>\lnot(\lnot p)\land \lnot q</m>.
    </p>

    <p>
      Using double negation, the expression simplifies to
      <m>p \land \lnot q</m>.
    </p>
  </solution>
</question>

  <!-- Question 3 -->
  <question xml:id="q-negation-billionaire">
    <statement>
      <p>
        Use logical equivalence to rewrite the statement:
        “It is not true that both you are a billionaire and I am crazy.”
      </p>
    </statement>
    <solution>
      <p>
        You are not a billionaire or I am not crazy.
      </p>
    </solution>
  </question>

  <!-- Question 4a -->
  <question xml:id="q-negation-wise-fool">
    <statement>
      <p>
        Use logical equivalence to rewrite the sentence:
        “It is not true that both I am wise and you are a fool.”
      </p>
    </statement>
    <solution>
      <p>
        I am not wise or you are not a fool.
      </p>
    </solution>
  </question>

  <!-- Question 4b -->
  <question xml:id="q-negation-either-wise-fool">
    <statement>
      <p>
        Use logical equivalence to rewrite the sentence:
        “It is not true that either I am wise or you are a fool.”
      </p>
    </statement>
    <solution>
      <p>
        I am not wise and you are not a fool.
      </p>
    </solution>
  </question>

  <!-- Question 4c -->
  <question xml:id="q-negation-conditional-party">
    <statement>
      <p>
        Use logical equivalence to rewrite the sentence:
        “If you decide to go to the party, then I will go with you.”
      </p>
    </statement>
    <solution>
      <p>
        If I do not go with you, then you did not decide to go to the party.
      </p>
    </solution>
  </question>

  <!-- Question 4d -->
  <question xml:id="q-negation-marriage">
    <statement>
      <p>
        Use logical equivalence to rewrite the sentence:
        “If you say ‘I do’, then you will be happy for the rest of your life.”
      </p>
    </statement>
    <solution>
      <p>
        If you are not happy for the rest of your life, then you did not say “I do.”
      </p>
    </solution>
  </question>

  <!-- Question 4e -->
  <question xml:id="q-negation-rug">
    <statement>
      <p>
        Use logical equivalence to rewrite the sentence:
        “I’ll be surprised if that is an authentic Persian rug.”
      </p>
    </statement>
    <solution>
      <p>
        If that is an authentic Persian rug, then I will be surprised.
      </p>
    </solution>
  </question>

  <!-- Question 4f -->
  <question xml:id="q-negation-peace">
    <statement>
      <p>
        Use logical equivalence to rewrite the sentence:
        “If wanting peace is wrong, I do not want to be right.”
      </p>
    </statement>
    <solution>
      <p>
        If I want to be right, then wanting peace is not wrong.
      </p>
    </solution>
  </question>

</subsection>

</section>