<?xml version="1.0" encoding="utf-8"?>
<section xml:id="section-course-requirements" xmlns:xi="http://www.w3.org/2001/XInclude">
  <title>Truth Tables</title>
<objectives xml:id="obj-ttable">
  <title>Goals for This Section</title>
  <ol>
    <li>
      Learn how to construct truth tables for statements.
    </li>
    <li>
    Learn <term>tautologies </term> and <term>contradictions</term>.
    </li>

  </ol>
</objectives>
<subsection>
  <title>Truth Tables</title>
  
  
<p>
  Each statement is True <term>T</term> or False <term>F</term>
  but not both. A truth table summarizes all possible truth values of a statement. 

</p>
<definition xml:id="def-ttablenegation">
  <statement>
    <p>
      Negation <term>reverses</term> the truth value of a statement.
    </p>
    <table>
  <title>Truth Table for Negation</title>
  <tabular halign="center">
    <row header="yes" bottom="minor">
      <cell><m>p</m></cell>
      <cell><m>\lnot p</m></cell>
    </row>
    <row>
      <cell>T</cell>
      <cell>F</cell>
    </row>
    <row>
      <cell>F</cell>
      <cell>T</cell>
    </row>
  </tabular>
</table>

  </statement>
</definition>
<definition xml:id="def-ttable-conjunction">
  <statement>
    <p>
      A <term>conjunction</term> (<m>\land</m>) combines two statements.
      The only case in which a conjunction is true is when
      <term>both statements are true</term>.
    </p>

    <table>
      <title>Truth Table for Conjunction</title>
      <tabular halign="center">
        <row header="yes" bottom="minor">
          <cell><m>p</m></cell>
          <cell><m>q</m></cell>
          <cell><m>p \land q</m></cell>
        </row>
        <row>
          <cell>T</cell>
          <cell>T</cell>
          <cell>T</cell>
        </row>
        <row>
          <cell>T</cell>
          <cell>F</cell>
          <cell>F</cell>
        </row>
        <row>
          <cell>F</cell>
          <cell>T</cell>
          <cell>F</cell>
        </row>
        <row>
          <cell>F</cell>
          <cell>F</cell>
          <cell>F</cell>
        </row>
      </tabular>
    </table>
  </statement>
</definition>
<definition xml:id="def-ttable-disjunction">
  <statement>
    <p>
      A <term>disjunction</term> (<m>\lor</m>) combines two statements.
      The only case in which a disjunction is <term>false</term>
      is when <term>both statements are false</term>.
    </p>

    <table>
      <title>Truth Table for Disjunction</title>
      <tabular halign="center">
        <row header="yes" bottom="minor">
          <cell><m>p</m></cell>
          <cell><m>q</m></cell>
          <cell><m>p \lor q</m></cell>
        </row>
        <row>
          <cell>T</cell>
          <cell>T</cell>
          <cell>T</cell>
        </row>
        <row>
          <cell>T</cell>
          <cell>F</cell>
          <cell>T</cell>
        </row>
        <row>
          <cell>F</cell>
          <cell>T</cell>
          <cell>T</cell>
        </row>
        <row>
          <cell>F</cell>
          <cell>F</cell>
          <cell>F</cell>
        </row>
      </tabular>
    </table>
  </statement>
</definition>
<example xml:id="ex-truthtable-demorgan-and">
  <title>Truth Table Practice</title>

  <statement>
    <p>
      Construct the truth table for the compound statement <m>\lnot(p \lor q) \land p</m>.
    </p>
  </statement>

  <solution>
    <p>
      Build the table by computing <m>p \lor q</m>, then <m>\lnot(p \lor q)</m>, and finally
      <m>\lnot(p \lor q) \land p</m>.
    </p>

    <table>
      <title>Truth Table for <m>\lnot(p \lor q) \land p</m></title>
      <tabular halign="center">
        <row header="yes" bottom="minor">
          <cell><m>p</m></cell>
          <cell><m>q</m></cell>
          <cell><m>p \lor q</m></cell>
          <cell><m>\lnot(p \lor q)</m></cell>
          <cell><m>\lnot(p \lor q)\land p</m></cell>
        </row>

        <row>
          <cell>T</cell>
          <cell>T</cell>
          <cell>T</cell>
          <cell>F</cell>
          <cell>F</cell>
        </row>

        <row>
          <cell>T</cell>
          <cell>F</cell>
          <cell>T</cell>
          <cell>F</cell>
          <cell>F</cell>
        </row>

        <row>
          <cell>F</cell>
          <cell>T</cell>
          <cell>T</cell>
          <cell>F</cell>
          <cell>F</cell>
        </row>

        <row>
          <cell>F</cell>
          <cell>F</cell>
          <cell>F</cell>
          <cell>T</cell>
          <cell>F</cell>
        </row>
      </tabular>
    </table>

    <p>
      The final column is always <m>F</m>, so the statement <m>\lnot(p \lor q) \land p</m>
      is a contradiction (always false).
    </p>
  </solution>
</example>
<definition xml:id="def-ttable-conditional">
  <statement>
    <p>
      A <term>conditional statement</term> is a compound statement of the form
      “if <m>p</m> then <m>q</m>,” written symbolically as <m>p \to q</m>.
      The statement <m>p</m> is called the <term>antecedent</term> (or condition),
      and the statement <m>q</m> is called the <term>consequent</term>.
    </p>

    <p>
      The only case in which a conditional statement is <term>false</term>
      is when the antecedent is <term>true</term> and the consequent is
      <term>false</term>.
    </p>

    <table>
      <title>Truth Table for Conditional</title>
      <tabular halign="center">
        <row header="yes" bottom="minor">
          <cell><m>p</m></cell>
          <cell><m>q</m></cell>
          <cell><m>p \to q</m></cell>
        </row>
        <row>
          <cell>T</cell>
          <cell>T</cell>
          <cell>T</cell>
        </row>
        <row>
          <cell>T</cell>
          <cell>F</cell>
          <cell>F</cell>
        </row>
        <row>
          <cell>F</cell>
          <cell>T</cell>
          <cell>T</cell>
        </row>
        <row>
          <cell>F</cell>
          <cell>F</cell>
          <cell>T</cell>
        </row>
      </tabular>
    </table>
  </statement>
</definition>
<exercise xml:id="ex-truthtable-conditional-conjunction">
  <title>Truth Table Practice</title>

  <statement>
    <p>
      Construct a truth table for the compound statement <m>(p \land q) \to q</m>.
    </p>
  </statement>

  <solution>
    <p>
      We first compute <m>p \land q</m>, and then evaluate the conditional
      <m>(p \land q) \to q</m>.
    </p>

    <table>
      <title>Truth Table for <m>(p \land q) \to q</m></title>
      <tabular halign="center">
        <row header="yes" bottom="minor">
          <cell><m>p</m></cell>
          <cell><m>q</m></cell>
          <cell><m>p \land q</m></cell>
          <cell><m>(p \land q) \to q</m></cell>
        </row>

        <row>
          <cell>T</cell>
          <cell>T</cell>
          <cell>T</cell>
          <cell>T</cell>
        </row>

        <row>
          <cell>T</cell>
          <cell>F</cell>
          <cell>F</cell>
          <cell>T</cell>
        </row>

        <row>
          <cell>F</cell>
          <cell>T</cell>
          <cell>F</cell>
          <cell>T</cell>
        </row>

        <row>
          <cell>F</cell>
          <cell>F</cell>
          <cell>F</cell>
          <cell>T</cell>
        </row>
      </tabular>
    </table>

    <p>
      Since the final column is always <m>T</m>, the statement
      <m>(p \land q) \to q</m> is a <term>tautology</term>.
    </p>
  </solution>
</exercise>
<remark xml:id="remark-conditional-variations">
  <title>Conditional Statement Variations</title>

  <p>
    A conditional statement of the form <m>p \to q</m> can be expressed in several
    equivalent ways in English. All of the following statements have the same logical
    meaning.
  </p>

  <ul>
    <li>If <m>p</m>, then <m>q</m>.</li>
    <li>If <m>p</m>, <m>q</m>.</li>
    <li><m>q</m> if <m>p</m>.</li>
    <li>When <m>p</m>, <m>q</m>.</li>
    <li><m>q</m> when <m>p</m>.</li>
    <li><m>p</m> is sufficient for <m>q</m>.</li>
    <li><m>q</m> is necessary for <m>p</m>.</li>
    <li><m>p</m> only if <m>q</m>.</li>
  </ul>
</remark>
<remark xml:id="remark-only-if-warning">
  <title>Common Pitfall: “If” vs. “Only If”</title>

  <p>
    A frequent source of confusion is the difference between the phrases
    <term>if</term> and <term>only if</term>.
  </p>

  <p>
    The statement “<m>p</m> only if <m>q</m>” means that <m>q</m> is
    <term>necessary</term> for <m>p</m>, and is translated symbolically as
    <m>p \to q</m>.
  </p>

  <p>
    In contrast, the statement “<m>p</m> if <m>q</m>” is translated as <m>q \to p</m>.
  </p>

  <p>
    One helpful rule to remember is:
  </p>

  <ul>
    <li>
      The phrase <term>only if</term> points to the <term>consequent</term>
      of a conditional statement.
    </li>
  </ul>

  <example xml:id="example-only-if">
    <title>Rewrite in if, then</title>
    <p>
      The statement “You pass the exam only if you attend class” means that
      attending class is necessary for passing the exam.
      Symbolically, this is written as <m>p \to q</m>, where
      <m>p</m> = “you pass the exam” and
      <m>q</m> = “you attend class.”
    </p>
  </example>
</remark>
<remark xml:id="remark-hidden-conditionals">
  <title>Hidden Conditional Statements in English</title>

  <p>
    Many statements in everyday English do not explicitly use the phrase
    “if … then …,” but they still express a conditional relationship.
    Such statements are called <term>hidden conditional statements</term>.
  </p>

  <p>
    In these cases, the conditional form can be revealed by rewriting the
    statement in an explicit “if … then …” format.
  </p>

  <example xml:id="example-hidden-conditional-koala">
    <title>Example</title>
    <p>
      The statement “No koalas live in South Carolina” can be rewritten as:
      “If it is a koala, then it does not live in South Carolina.”
    </p>
  </example>

  <example xml:id="example-hidden-conditional-jordan">
    <title>Example</title>
    <p>
      The statement “Michael Jordan eats Wheaties” can be rewritten as:
      “If you are Michael Jordan, then you eat Wheaties.”
    </p>
  </example>

</remark>
<exercise xml:id="ex-rewrite-if-then">
  <title>Rewriting Statements as Conditionals</title>


  <task xml:id="task-rewrite-if-then-a">
    <statement> 
    <p>
      Rewrite the following statement using the form <em>if … then …</em>.
    </p>

      <p> Every picture tells a story.</p>
    </statement>
    <solution>
      <p>If it is a picture, then it tells a story.</p>
    </solution>
  </task>

  <task xml:id="task-rewrite-if-then-b">
    <statement>
          <p>
      Rewrite the following statement using the form <em>if … then …</em>.
    </p>
      <p> I can come with you only if I can find some time.</p>
    </statement>
    <solution>
      <p>If I can come with you, then I can find some time.</p>
    </solution>
  </task>

</exercise>
<example xml:id="example-truthtable-three-variables">
  <title>Truth Table with Three Variables</title>

  <p>
    Consider the compound statement <m>(p \land q) \lor \lnot r</m>, which involves
    three simple statements: <m>p</m>, <m>q</m>, and <m>r</m>.
  </p>

  <p>
    Compound statements may contain several simple statements. In order to determine
    how many columns are needed in a truth table, it is helpful to break the compound
    statement into <term>building blocks</term> of increasing complexity, starting
    with a column for each simple statement and ending with the compound statement
    itself.
  </p>

  <p>
    For this example, the building blocks are:
  </p>

  <ul>
    <li><m>p</m></li>
    <li><m>q</m></li>
    <li><m>r</m></li>
    <li><m>p \land q</m></li>
    <li><m>\lnot r</m></li>
    <li><m>(p \land q) \lor \lnot r</m></li>
  </ul>

  <solution>
    <table>
      <title>Truth Table for <m>(p \land q) \lor \lnot r</m></title>
      <tabular halign="center">
        <row header="yes" bottom="minor">
          <cell><m>p</m></cell>
          <cell><m>q</m></cell>
          <cell><m>r</m></cell>
          <cell><m>p \land q</m></cell>
          <cell><m>\lnot r</m></cell>
          <cell><m>(p \land q) \lor \lnot r</m></cell>
        </row>

        <row>
          <cell>T</cell><cell>T</cell><cell>T</cell>
          <cell>T</cell><cell>F</cell><cell>T</cell>
        </row>
        <row>
          <cell>T</cell><cell>T</cell><cell>F</cell>
          <cell>T</cell><cell>T</cell><cell>T</cell>
        </row>
        <row>
          <cell>T</cell><cell>F</cell><cell>T</cell>
          <cell>F</cell><cell>F</cell><cell>F</cell>
        </row>
        <row>
          <cell>T</cell><cell>F</cell><cell>F</cell>
          <cell>F</cell><cell>T</cell><cell>T</cell>
        </row>
        <row>
          <cell>F</cell><cell>T</cell><cell>T</cell>
          <cell>F</cell><cell>F</cell><cell>F</cell>
        </row>
        <row>
          <cell>F</cell><cell>T</cell><cell>F</cell>
          <cell>F</cell><cell>T</cell><cell>T</cell>
        </row>
        <row>
          <cell>F</cell><cell>F</cell><cell>T</cell>
          <cell>F</cell><cell>F</cell><cell>F</cell>
        </row>
        <row>
          <cell>F</cell><cell>F</cell><cell>F</cell>
          <cell>F</cell><cell>T</cell><cell>T</cell>
        </row>
      </tabular>
    </table>

    <p>
      By constructing the truth table one building block at a time, we reduce errors
      and make the logical structure of the compound statement clear.
    </p>
  </solution>
</example>
</subsection>
<subsection xml:id="subsec-exercises-truth-tables">
  <title>Exercises</title>

  <p>
    Construct truth tables for the following compound statements.
    Include columns for each simple statement and each intermediate component,
    ending with the compound statement itself.
  </p>

  <!-- (a) p ∧ ¬q -->
  <question xml:id="q-tt-a">
    <statement><p>Construct a truth table for <m>p \land \lnot q</m>.</p></statement>
    <solution>
      <table>
        <title>Truth Table for <m>p \land \lnot q</m></title>
        <tabular halign="center">
          <row header="yes" bottom="minor">
            <cell><m>p</m></cell>
            <cell><m>q</m></cell>
            <cell><m>\lnot q</m></cell>
            <cell><m>p \land \lnot q</m></cell>
          </row>
          <row><cell>T</cell><cell>T</cell><cell>F</cell><cell>F</cell></row>
          <row><cell>T</cell><cell>F</cell><cell>T</cell><cell>T</cell></row>
          <row><cell>F</cell><cell>T</cell><cell>F</cell><cell>F</cell></row>
          <row><cell>F</cell><cell>F</cell><cell>T</cell><cell>F</cell></row>
        </tabular>
      </table>
    </solution>
  </question>

  <!-- (b) ¬(¬p) ∧ p -->
  <question xml:id="q-tt-b">
    <statement><p>Construct a truth table for <m>\lnot(\lnot p) \land p</m>.</p></statement>
    <solution>
      <table>
        <title>Truth Table for <m>\lnot(\lnot p) \land p</m></title>
        <tabular halign="center">
          <row header="yes" bottom="minor">
            <cell><m>p</m></cell>
            <cell><m>\lnot p</m></cell>
            <cell><m>\lnot(\lnot p)</m></cell>
            <cell><m>\lnot(\lnot p)\land p</m></cell>
          </row>
          <row><cell>T</cell><cell>F</cell><cell>T</cell><cell>T</cell></row>
          <row><cell>F</cell><cell>T</cell><cell>F</cell><cell>F</cell></row>
        </tabular>
      </table>
    </solution>
  </question>

  <!-- (c) ¬(p ∨ q) -->
  <question xml:id="q-tt-c">
    <statement><p>Construct a truth table for <m>\lnot(p \lor q)</m>.</p></statement>
    <solution>
      <table>
        <title>Truth Table for <m>\lnot(p \lor q)</m></title>
        <tabular halign="center">
          <row header="yes" bottom="minor">
            <cell><m>p</m></cell>
            <cell><m>q</m></cell>
            <cell><m>p \lor q</m></cell>
            <cell><m>\lnot(p \lor q)</m></cell>
          </row>
          <row><cell>T</cell><cell>T</cell><cell>T</cell><cell>F</cell></row>
          <row><cell>T</cell><cell>F</cell><cell>T</cell><cell>F</cell></row>
          <row><cell>F</cell><cell>T</cell><cell>T</cell><cell>F</cell></row>
          <row><cell>F</cell><cell>F</cell><cell>F</cell><cell>T</cell></row>
        </tabular>
      </table>
    </solution>
  </question>

  <!-- (d) (¬p) ∧ ¬q -->
  <question xml:id="q-tt-d">
    <statement><p>Construct a truth table for <m>(\lnot p)\land \lnot q</m>.</p></statement>
    <solution>
      <table>
        <title>Truth Table for <m>(\lnot p)\land \lnot q</m></title>
        <tabular halign="center">
          <row header="yes" bottom="minor">
            <cell><m>p</m></cell>
            <cell><m>q</m></cell>
            <cell><m>\lnot p</m></cell>
            <cell><m>\lnot q</m></cell>
            <cell><m>(\lnot p)\land \lnot q</m></cell>
          </row>
          <row><cell>T</cell><cell>T</cell><cell>F</cell><cell>F</cell><cell>F</cell></row>
          <row><cell>T</cell><cell>F</cell><cell>F</cell><cell>T</cell><cell>F</cell></row>
          <row><cell>F</cell><cell>T</cell><cell>T</cell><cell>F</cell><cell>F</cell></row>
          <row><cell>F</cell><cell>F</cell><cell>T</cell><cell>T</cell><cell>T</cell></row>
        </tabular>
      </table>
    </solution>
  </question>

  <!-- (e) ¬(p ∨ ¬q) ∨ p -->
  <question xml:id="q-tt-e">
    <statement><p>Construct a truth table for <m>\lnot(p \lor \lnot q)\lor p</m>.</p></statement>
    <solution>
      <table>
        <title>Truth Table for <m>\lnot(p \lor \lnot q)\lor p</m></title>
        <tabular halign="center">
          <row header="yes" bottom="minor">
            <cell><m>p</m></cell>
            <cell><m>q</m></cell>
            <cell><m>\lnot q</m></cell>
            <cell><m>p \lor \lnot q</m></cell>
            <cell><m>\lnot(p \lor \lnot q)</m></cell>
            <cell><m>\lnot(p \lor \lnot q)\lor p</m></cell>
          </row>
          <row><cell>T</cell><cell>T</cell><cell>F</cell><cell>T</cell><cell>F</cell><cell>T</cell></row>
          <row><cell>T</cell><cell>F</cell><cell>T</cell><cell>T</cell><cell>F</cell><cell>T</cell></row>
          <row><cell>F</cell><cell>T</cell><cell>F</cell><cell>F</cell><cell>T</cell><cell>T</cell></row>
          <row><cell>F</cell><cell>F</cell><cell>T</cell><cell>T</cell><cell>F</cell><cell>F</cell></row>
        </tabular>
      </table>
    </solution>
  </question>

  <!-- (f) ¬(p ∨ (¬q)) ∧ r -->
  <question xml:id="q-tt-f">
    <statement><p>Construct a truth table for <m>\lnot(p \lor (\lnot q))\land r</m>.</p></statement>
    <solution>
      <table>
        <title>Truth Table for <m>\lnot(p \lor (\lnot q))\land r</m></title>
        <tabular halign="center">
          <row header="yes" bottom="minor">
            <cell><m>p</m></cell>
            <cell><m>q</m></cell>
            <cell><m>r</m></cell>
            <cell><m>\lnot q</m></cell>
            <cell><m>p \lor (\lnot q)</m></cell>
            <cell><m>\lnot(p \lor (\lnot q))</m></cell>
            <cell><m>\lnot(p \lor (\lnot q))\land r</m></cell>
          </row>
          <row><cell>T</cell><cell>T</cell><cell>T</cell><cell>F</cell><cell>T</cell><cell>F</cell><cell>F</cell></row>
          <row><cell>T</cell><cell>T</cell><cell>F</cell><cell>F</cell><cell>T</cell><cell>F</cell><cell>F</cell></row>
          <row><cell>T</cell><cell>F</cell><cell>T</cell><cell>T</cell><cell>T</cell><cell>F</cell><cell>F</cell></row>
          <row><cell>T</cell><cell>F</cell><cell>F</cell><cell>T</cell><cell>T</cell><cell>F</cell><cell>F</cell></row>
          <row><cell>F</cell><cell>T</cell><cell>T</cell><cell>F</cell><cell>F</cell><cell>T</cell><cell>T</cell></row>
          <row><cell>F</cell><cell>T</cell><cell>F</cell><cell>F</cell><cell>F</cell><cell>T</cell><cell>F</cell></row>
          <row><cell>F</cell><cell>F</cell><cell>T</cell><cell>T</cell><cell>T</cell><cell>F</cell><cell>F</cell></row>
          <row><cell>F</cell><cell>F</cell><cell>F</cell><cell>T</cell><cell>T</cell><cell>F</cell><cell>F</cell></row>
        </tabular>
      </table>
    </solution>
  </question>

  <!-- (g) (r ∧ p) ∨ ¬q -->
  <question xml:id="q-tt-g">
    <statement><p>Construct a truth table for <m>(r \land p)\lor \lnot q</m>.</p></statement>
    <solution>
      <table>
        <title>Truth Table for <m>(r \land p)\lor \lnot q</m></title>
        <tabular halign="center">
          <row header="yes" bottom="minor">
            <cell><m>p</m></cell>
            <cell><m>q</m></cell>
            <cell><m>r</m></cell>
            <cell><m>r \land p</m></cell>
            <cell><m>\lnot q</m></cell>
            <cell><m>(r \land p)\lor \lnot q</m></cell>
          </row>
          <row><cell>T</cell><cell>T</cell><cell>T</cell><cell>T</cell><cell>F</cell><cell>T</cell></row>
          <row><cell>T</cell><cell>T</cell><cell>F</cell><cell>F</cell><cell>F</cell><cell>F</cell></row>
          <row><cell>T</cell><cell>F</cell><cell>T</cell><cell>T</cell><cell>T</cell><cell>T</cell></row>
          <row><cell>T</cell><cell>F</cell><cell>F</cell><cell>F</cell><cell>T</cell><cell>T</cell></row>
          <row><cell>F</cell><cell>T</cell><cell>T</cell><cell>F</cell><cell>F</cell><cell>F</cell></row>
          <row><cell>F</cell><cell>T</cell><cell>F</cell><cell>F</cell><cell>F</cell><cell>F</cell></row>
          <row><cell>F</cell><cell>F</cell><cell>T</cell><cell>F</cell><cell>T</cell><cell>T</cell></row>
          <row><cell>F</cell><cell>F</cell><cell>F</cell><cell>F</cell><cell>T</cell><cell>T</cell></row>
        </tabular>
      </table>
    </solution>
  </question>
<!-- (h) (p ∧ q) → q -->
<question xml:id="q-tt-h">
  <statement>
    <p>Construct a truth table for <m>(p \land q)\to q</m>.</p>
  </statement>
  <solution>
    <table>
      <title>Truth Table for <m>(p \land q)\to q</m></title>
      <tabular halign="center">
        <row header="yes" bottom="minor">
          <cell><m>p</m></cell>
          <cell><m>q</m></cell>
          <cell><m>p \land q</m></cell>
          <cell><m>(p \land q)\to q</m></cell>
        </row>
        <row><cell>T</cell><cell>T</cell><cell>T</cell><cell>T</cell></row>
        <row><cell>T</cell><cell>F</cell><cell>F</cell><cell>T</cell></row>
        <row><cell>F</cell><cell>T</cell><cell>F</cell><cell>T</cell></row>
        <row><cell>F</cell><cell>F</cell><cell>F</cell><cell>T</cell></row>
      </tabular>
    </table>
  </solution>
</question>

<!-- (i) (¬p) → (p → q) -->
<question xml:id="q-tt-i">
  <statement>
    <p>Construct a truth table for <m>(\lnot p)\to (p\to q)</m>.</p>
  </statement>
  <solution>
    <table>
      <title>Truth Table for <m>(\lnot p)\to (p\to q)</m></title>
      <tabular halign="center">
        <row header="yes" bottom="minor">
          <cell><m>p</m></cell>
          <cell><m>q</m></cell>
          <cell><m>\lnot p</m></cell>
          <cell><m>p\to q</m></cell>
          <cell><m>(\lnot p)\to (p\to q)</m></cell>
        </row>
        <row><cell>T</cell><cell>T</cell><cell>F</cell><cell>T</cell><cell>T</cell></row>
        <row><cell>T</cell><cell>F</cell><cell>F</cell><cell>F</cell><cell>T</cell></row>
        <row><cell>F</cell><cell>T</cell><cell>T</cell><cell>T</cell><cell>T</cell></row>
        <row><cell>F</cell><cell>F</cell><cell>T</cell><cell>T</cell><cell>T</cell></row>
      </tabular>
    </table>
  </solution>
</question>

<!-- (j) [p ∧ (¬q ∨ r)] → (q ∨ ¬p) -->
<question xml:id="q-tt-j">
  <statement>
    <p>
      Construct a truth table for
      <m>[p \land (\lnot q \lor r)] \to (q \lor \lnot p)</m>.
    </p>
  </statement>
  <solution>
    <table>
      <title>Truth Table for <m>[p \land (\lnot q \lor r)] \to (q \lor \lnot p)</m></title>
      <tabular halign="center">
        <row header="yes" bottom="minor">
          <cell><m>p</m></cell>
          <cell><m>q</m></cell>
          <cell><m>r</m></cell>
          <cell><m>\lnot q</m></cell>
          <cell><m>\lnot q \lor r</m></cell>
          <cell><m>p \land (\lnot q \lor r)</m></cell>
          <cell><m>\lnot p</m></cell>
          <cell><m>q \lor \lnot p</m></cell>
          <cell><m>[p \land (\lnot q \lor r)] \to (q \lor \lnot p)</m></cell>
        </row>

        <row><cell>T</cell><cell>T</cell><cell>T</cell><cell>F</cell><cell>T</cell><cell>T</cell><cell>F</cell><cell>T</cell><cell>T</cell></row>
        <row><cell>T</cell><cell>T</cell><cell>F</cell><cell>F</cell><cell>F</cell><cell>F</cell><cell>F</cell><cell>T</cell><cell>T</cell></row>
        <row><cell>T</cell><cell>F</cell><cell>T</cell><cell>T</cell><cell>T</cell><cell>T</cell><cell>F</cell><cell>F</cell><cell>F</cell></row>
        <row><cell>T</cell><cell>F</cell><cell>F</cell><cell>T</cell><cell>T</cell><cell>T</cell><cell>F</cell><cell>F</cell><cell>F</cell></row>
        <row><cell>F</cell><cell>T</cell><cell>T</cell><cell>F</cell><cell>T</cell><cell>F</cell><cell>T</cell><cell>T</cell><cell>T</cell></row>
        <row><cell>F</cell><cell>T</cell><cell>F</cell><cell>F</cell><cell>F</cell><cell>F</cell><cell>T</cell><cell>T</cell><cell>T</cell></row>
        <row><cell>F</cell><cell>F</cell><cell>T</cell><cell>T</cell><cell>T</cell><cell>F</cell><cell>T</cell><cell>T</cell><cell>T</cell></row>
        <row><cell>F</cell><cell>F</cell><cell>F</cell><cell>T</cell><cell>T</cell><cell>F</cell><cell>T</cell><cell>T</cell><cell>T</cell></row>
      </tabular>
    </table>
  </solution>
</question>

</subsection>
<subsection xml:id="subsec-">
  <title>Tautology and Contradiction</title>
  <p>
    A <term>tautology</term> is a statement that is always true. 
  </p>
<p>
A <term>contradiction</term> is a statement that are always false. 

  </p>
  <exercise xml:id="ex-tautology-contradiction">
  <title>Tautology and Contradiction</title>

  <statement>
    <p>
      For each statement, construct a truth table (including columns for intermediate
      components) and use the final column to determine whether the statement is a
      <term>tautology</term> or a <term>contradiction</term>.
    </p>
  </statement>

  <!-- Tautology -->
  <task xml:id="task-tautology-1">
    <statement>
      <p>
        Show that the statement <m>p \lor \lnot(p \lor q)</m> is a tautology by constructing its truth table.
      </p>
    </statement>
    <solution>
      <table>
        <title>Truth Table for <m>p \lor \lnot(p \lor q)</m></title>
        <tabular halign="center">
          <row header="yes" bottom="minor">
            <cell><m>p</m></cell>
            <cell><m>q</m></cell>
            <cell><m>p \lor q</m></cell>
            <cell><m>\lnot(p \lor q)</m></cell>
            <cell><m>p \lor \lnot(p \lor q)</m></cell>
          </row>
          <row><cell>T</cell><cell>T</cell><cell>T</cell><cell>F</cell><cell>T</cell></row>
          <row><cell>T</cell><cell>F</cell><cell>T</cell><cell>F</cell><cell>T</cell></row>
          <row><cell>F</cell><cell>T</cell><cell>T</cell><cell>F</cell><cell>F</cell></row>
          <row><cell>F</cell><cell>F</cell><cell>F</cell><cell>T</cell><cell>T</cell></row>
        </tabular>
      </table>
      <p>
        Since the final column is not always <m>T</m>, this statement is <em>not</em> a tautology.
      </p>
    </solution>
  </task>

  <!-- Tautology (actually a tautology) -->
  <task xml:id="task-tautology-2">
    <statement>
      <p>
        Show that the statement <m>(p \land q)\to p</m> is a tautology by constructing its truth table.
      </p>
    </statement>
    <solution>
      <table>
        <title>Truth Table for <m>(p \land q)\to p</m></title>
        <tabular halign="center">
          <row header="yes" bottom="minor">
            <cell><m>p</m></cell>
            <cell><m>q</m></cell>
            <cell><m>p \land q</m></cell>
            <cell><m>(p \land q)\to p</m></cell>
          </row>
          <row><cell>T</cell><cell>T</cell><cell>T</cell><cell>T</cell></row>
          <row><cell>T</cell><cell>F</cell><cell>F</cell><cell>T</cell></row>
          <row><cell>F</cell><cell>T</cell><cell>F</cell><cell>T</cell></row>
          <row><cell>F</cell><cell>F</cell><cell>F</cell><cell>T</cell></row>
        </tabular>
      </table>
      <p>
        The final column is always <m>T</m>, so the statement is a tautology.
      </p>
    </solution>
  </task>

  <!-- Contradiction -->
  <task xml:id="task-contradiction-1">
    <statement>
      <p>
        Show that the statement <m>p \land \lnot p</m> is a contradiction by constructing its truth table.
      </p>
    </statement>
    <solution>
      <table>
        <title>Truth Table for <m>p \land \lnot p</m></title>
        <tabular halign="center">
          <row header="yes" bottom="minor">
            <cell><m>p</m></cell>
            <cell><m>\lnot p</m></cell>
            <cell><m>p \land \lnot p</m></cell>
          </row>
          <row><cell>T</cell><cell>F</cell><cell>F</cell></row>
          <row><cell>F</cell><cell>T</cell><cell>F</cell></row>
        </tabular>
      </table>
      <p>
        The final column is always <m>F</m>, so the statement is a contradiction.
      </p>
    </solution>
  </task>

</exercise>

</subsection>
</section>

